cfrontend/SimplLocalsproof.v
@@ -315,7 +315,7 @@ Lemma step_Sset_debug:
   forall f id ty a k e le m v v',
   eval_expr tge e le m a v ->
   sem_cast v (typeof a) ty m = Some v' ->
-  plus step2 tge (State f (Sset_debug id ty a) k e le m)
+  plus (step2 tge) (State f (Sset_debug id ty a) k e le m)
               E0 (State f Sskip k e (PTree.set id v' le) m).
 Proof.
   intros; unfold Sset_debug.
@@ -335,7 +335,7 @@ Qed.
 Lemma step_add_debug_vars:
   forall f s e le m vars k,
   (forall id ty, In (id, ty) vars -> exists b, e!id = Some (b, ty)) ->
-  star step2 tge (State f (add_debug_vars vars s) k e le m)
+  star (step2 tge) (State f (add_debug_vars vars s) k e le m)
               E0 (State f s k e le m).
 Proof.
   unfold add_debug_vars. destruct (Compopts.debug tt).
@@ -369,7 +369,7 @@ Lemma step_add_debug_params:
   list_norepet (var_names params) ->
   list_forall2 val_casted vl (map snd params) ->
   bind_parameter_temps params vl le1 = Some le ->
-  star step2 tge (State f (add_debug_params params s) k e le m)
+  star (step2 tge) (State f (add_debug_params params s) k e le m)
               E0 (State f s k e le m).
 Proof.
   unfold add_debug_params. destruct (Compopts.debug tt).
@@ -1102,7 +1102,7 @@ Theorem store_params_correct:
   (forall id, ~In id (var_names params) -> tle2!id = tle1!id) ->
   (forall id, In id (var_names params) -> le!id = None) ->
   exists tle, exists tm',
-  star step2 tge (State f (store_params cenv params s) k te tle tm)
+  star (step2 tge) (State f (store_params cenv params s) k te tle tm)
               E0 (State f s k te tle tm')
   /\ bind_parameter_temps params targs tle2 = Some tle
   /\ Mem.inject j m' tm'
@@ -2002,7 +2002,7 @@ End FIND_LABEL.
 
 Lemma step_simulation:
   forall S1 t S2, step1 ge S1 t S2 ->
-  forall S1' (MS: match_states S1 S1'), exists S2', plus step2 tge S1' t S2' /\ match_states S2 S2'.
+  forall S1' (MS: match_states S1 S1'), exists S2', plus (step2 tge) S1' t S2' /\ match_states S2 S2'.
 Proof.
   induction 1; simpl; intros; inv MS; simpl in *; try (monadInv TRS).
 
@@ -2242,8 +2242,8 @@ Qed.
 
 
 Lemma entry_points_simulation:
-  forall S v args m, entry_point prog m S v args ->
-       exists R, entry_point tprog m R v args /\ match_states S R.
+  forall g S v args m, entry_point g m S v args ->
+       exists R, entry_point g m R v args /\ match_states S R.
 Proof.
   intros. inv H.
   exploit function_ptr_translated; eauto. intros [tf [A B]].
